src/crypto_foundations/primitives/signature.lean
@@ -8,6 +8,7 @@ import computational_monads.coercions.sim_oracle
 import computational_monads.asymptotics.polynomial_time
 import computational_monads.asymptotics.negligable
 import computational_monads.asymptotics.queries_at_most
+import computational_monads.simulation_semantics.oracle_append
 
 /-!
 # Cryptographic Signature Schemes
